src/riscv/Utility/RecordSetters.v
@@ -1,0 +1,262 @@
+Require Import Ltac2.Ltac2.
+Require Ltac2.Option.
+Set Default Proof Mode "Classic".
+
+Ltac2 rec strip_foralls(t: constr) :=
+  match Constr.Unsafe.kind t with
+  | Constr.Unsafe.Prod b u => let (bs, body) := strip_foralls u in (b :: bs, body)
+  | _ => ([], t)
+  end.
+
+Ltac2 app_arg_count(t: constr) :=
+  match Constr.Unsafe.kind t with
+  | Constr.Unsafe.App f args => Array.length args
+  | _ => 0
+  end.
+
+Ltac2 binder_to_field(qualification: ident list)(b: binder) :=
+   Option.get (Env.get (List.append qualification [Option.get (Constr.Binder.name b)])).
+
+Ltac2 field_names(ctor_ref: Std.reference) :=
+  let ctor_type := Constr.type (Env.instantiate ctor_ref) in
+  let (binders, result) := strip_foralls ctor_type in
+  let n_type_args := app_arg_count result in
+  let field_name_binders := List.skipn n_type_args binders in
+  List.map (binder_to_field (List.removelast (Env.path ctor_ref))) field_name_binders.
+
+Ltac2 constructor_of_record(t: constr) :=
+  match Constr.Unsafe.kind t with
+  | Constr.Unsafe.Ind ind inst =>
+    Std.ConstructRef (Constr.Unsafe.constructor ind 0)
+  | _ => Control.throw (Invalid_argument (Some (Message.of_constr t)))
+  end.
+
+Ltac2 mkApp(f: constr)(args: constr array) :=
+  Constr.Unsafe.make (Constr.Unsafe.App f args).
+
+Ltac2 eta(t: constr) :=
+  let (h, args) := match Constr.Unsafe.kind t with
+                   | Constr.Unsafe.App h args => (h, args)
+                   | _ => (t, Array.empty ())
+                   end in
+  let ctor := constructor_of_record h in
+  let getters := List.map (fun getterRef => mkApp (Env.instantiate getterRef) args)
+                          (field_names ctor) in
+  constr:(fun x: $t => ltac2:(
+    let projections := List.map (fun getter => constr:($getter &x)) getters in
+    let res := mkApp (mkApp (Env.instantiate ctor) args) (Array.of_list projections) in
+    exact $res)).
+
+Ltac exact_eta :=
+  ltac2:(t |- let res := eta (Option.get (Ltac1.to_constr t)) in exact $res).
+
+Ltac eta T := constr:(ltac:(exact_eta T)).
+
+Definition Updater{R E: Type}(getter: R -> E): Type := (E -> E) -> R -> R.
+Existing Class Updater.
+
+Ltac updater R getter :=
+  let etaR := eta R in
+  lazymatch etaR with
+  | context[getter] => idtac
+  | _ => fail 1 getter "is not a field of" R
+  end;
+  lazymatch eval pattern getter in etaR with
+  | ?updateR _ =>
+      let u := eval cbv beta in (fun updateE => updateR (fun r => updateE (getter r))) in
+      exact u
+  end.
+
+Global Hint Extern 1 (@Updater ?R ?E ?getter) => updater R getter : typeclass_instances.
+
+(* Note: in coq-record-update, the second-to-last argument of `set` is an updater
+   of type `E -> E` (a function transforming an old value into a new value),
+   and for setting a field, it just passes a constant function that ignores the
+   old value.
+   This is inconvenient for me because I use rewriting/simplification tactics that
+   don't recurse under binders, but I do want them to recurse into new values of set,
+   so we need two separate definitions for `set` and `update` *)
+
+Definition update{R E: Type}(getter: R -> E){updater: Updater getter}
+  : (E -> E) -> R -> R := updater.
+
+Definition set{R E: Type}(getter: R -> E){updater: Updater getter}(newVal: E): R -> R :=
+  updater (fun _ => newVal).
+
+(*
+Module RecordSetNotations1.
+  Declare Scope record_set.
+  Delimit Scope record_set with rs.
+  Open Scope rs.
+  (* Note: coq-record-update uses level 12, but I prefer level 8:
+      https://github.com/tchajed/coq-record-update/issues/14 *)
+  Notation "x <| proj ::= f |>" := (update proj f x)
+     (at level 8, f at next level, left associativity, format "x <| proj  ::=  f |>")
+     : record_set.
+  Notation "x <| proj := v |>" := (set proj v x)
+     (at level 8, left associativity, format "x <| proj  :=  v |>")
+     : record_set.
+End RecordSetNotations1.
+*)
+
+Module Export RecordSetNotationsOCamlLike.
+  Declare Scope record_set.
+  Delimit Scope record_set with rs.
+  Open Scope rs.
+
+  Declare Custom Entry field_update.
+  Notation "proj := v" := (set proj v)
+    (in custom field_update at level 1, proj constr at level 99, v constr at level 99)
+    : record_set.
+  Notation "proj ::= f" := (update proj f)
+    (in custom field_update at level 1, proj constr at level 99, f constr at level 99)
+    : record_set.
+
+  (* marker function to enable notation printing *)
+  Definition apply_update{R: Type}(u: R -> R): R -> R := u.
+
+  Notation "{ x 'with' u }" := (apply_update u x)
+     (at level 0, x at level 99, u custom field_update at level 1,
+      format "{  x  'with'  u  }") : record_set.
+  Notation "{ x 'with' u ; .. ; v ; w }" :=
+     (apply_update w (apply_update v .. (apply_update u x) .. ))
+     (at level 0, x at level 99, u custom field_update at level 1,
+      v custom field_update at level 1, w custom field_update at level 1,
+      format "{  x  'with'  u ;  .. ;  v ;  w  }") : record_set.
+End RecordSetNotationsOCamlLike.
+
+Module LeftUpdateNotations.
+  Declare Scope record_set.
+  Delimit Scope record_set with rs.
+  Open Scope rs.
+
+  Declare Custom Entry fld_update.
+  Notation "proj := v" := (set proj v)
+    (in custom fld_update at level 1, proj constr at level 99, v constr at level 99)
+    : record_set.
+  Notation "proj ::= f" := (update proj f)
+    (in custom fld_update at level 1, proj constr at level 99, f constr at level 99)
+    : record_set.
+  Notation "'{!' u }" := u
+     (at level 0, u custom fld_update at level 1,
+      format "'{!'  u  }")
+    : record_set.
+  Notation "'{!' u ; v ; .. ; w } r" := (u (v .. (w r) ..))
+     (at level 10, u custom fld_update at level 1, r constr at level 9,
+      v custom fld_update at level 1, w custom fld_update at level 1,
+      format "'{!'  u ;  v ;  .. ;  w  }  r")
+    : record_set.
+  (* Doesn't print. If move the r into (fun r => ...) on the rhs, it prints, but as
+     soon as a `cbv beta` happens, it doesn't print any more *)
+End LeftUpdateNotations.
+
+Module RecordSetterTests.
+
+  Record foo(A: Type)(n: nat) := {
+    fieldA: A;
+    fieldB: n = n;
+    fieldC: bool;
+  }.
+
+  Arguments fieldA {_ _}.
+  Arguments fieldB {_ _}.
+  Arguments fieldC {_ _}.
+
+  Example testFoo(b: bool): foo nat 2 :=
+    {| fieldA := 3; fieldB := eq_refl; fieldC := b |}.
+
+  Goal forall b, { testFoo b with fieldC := false } = { testFoo b with fieldC := false }.
+  Abort.
+
+  Goal forall b,
+      { testFoo b with fieldC := true; fieldC := false; fieldA ::= Nat.add 2 } =
+      { testFoo b with fieldA ::= Nat.add 1; fieldC := false; fieldA ::= Nat.add 1 }.
+  Proof.
+    intros. unfold apply_update. unfold update, set. cbn. reflexivity.
+  Qed.
+End RecordSetterTests.
+
+
+Module record.
+
+  Ltac head t :=
+    lazymatch t with
+    | ?f _ => head f
+    | _ => t
+    end.
+
+  Ltac apply_set fullRecord partialRecord getter newVal :=
+    match partialRecord with
+    | ?rest ?fieldVal =>
+        let __ := match constr:(Set) with
+                  | _ => unify (getter fullRecord) fieldVal
+                  end in
+        constr:(rest newVal)
+    | ?rest ?fieldVal =>
+        let r := apply_set fullRecord rest getter newVal in constr:(r fieldVal)
+    end.
+
+  (* TODO generalize: ltac that traverses list of updates and unique-ifies them *)
+  Ltac simp_step :=
+    match goal with
+    | |- context[ ?fieldA { ?r with ?fieldB := ?v } ] =>
+        progress tryif constr_eq fieldA fieldB
+        then change (fieldA { r with fieldB := v }) with v
+        else change (fieldA { r with fieldB := v }) with (fieldA r)
+    | |- context[ ?fieldA { ?r with ?fieldB ::= ?f } ] =>
+        progress tryif constr_eq fieldA fieldB
+        then change (fieldA { r with fieldB ::= f }) with (f (fieldA r))
+        else change (fieldA { r with fieldB ::= f }) with (fieldA r)
+    | |- context[{ ?r with ?field := ?v1; ?field := ?v2 }] =>
+        progress change { r with field := v1; field := v2 } with { r with field := v2 }
+    | |- context[{ ?r with ?field ::= ?f1; ?field := ?v2 }] =>
+        progress change { r with field ::= f1; field := v2 } with { r with field := v2 }
+    | |- context[{ ?r with ?field := ?v1; ?field ::= ?f2 }] =>
+        progress change { r with field := v1; field ::= f2 }
+                 with { r with field := f2 v1 }
+    | |- context[{ ?r with ?field ::= ?f1; ?field ::= ?f2 }] =>
+        progress change { r with field ::= f1; field ::= f2 }
+                 with { r with field := f2 (f1 (field r)) }
+    | |- context[{ ?r with ?field := ?v }] =>
+        let h := head r in is_constructor h;
+        let res := apply_set r r field v in
+        progress change { r with field := v } with res
+    | |- context[{ ?r with ?field ::= ?f }] =>
+        let h := head r in is_constructor h;
+        let bare_field := head field in (* <-- strip implicit args/params *)
+        let oldval := eval cbn [bare_field] in (field r) in
+        let res := apply_set r r field (f oldval) in
+        progress change { r with field ::= f } with res
+
+    | H: context[ ?fieldA { ?r with ?fieldB := ?v } ] |- _ =>
+        progress tryif constr_eq fieldA fieldB
+        then change (fieldA { r with fieldB := v }) with v in H
+        else change (fieldA { r with fieldB := v }) with (fieldA r) in H
+    | H: context[ ?fieldA { ?r with ?fieldB ::= ?f } ] |- _ =>
+        progress tryif constr_eq fieldA fieldB
+        then change (fieldA { r with fieldB ::= f }) with (f (fieldA r)) in H
+        else change (fieldA { r with fieldB ::= f }) with (fieldA r) in H
+    | H: context[{ ?r with ?field := ?v1; ?field := ?v2 }] |- _ =>
+        progress change { r with field := v1; field := v2 } with { r with field := v2 } in H
+    | H: context[{ ?r with ?field ::= ?f1; ?field := ?v2 }] |- _ =>
+        progress change { r with field ::= f1; field := v2 } with { r with field := v2 } in H
+    | H: context[{ ?r with ?field := ?v1; ?field ::= ?f2 }] |- _ =>
+        progress change { r with field := v1; field ::= f2 }
+                 with { r with field := f2 v1 } in H
+    | H: context[{ ?r with ?field ::= ?f1; ?field ::= ?f2 }] |- _ =>
+        progress change { r with field ::= f1; field ::= f2 }
+                 with { r with field := f2 (f1 (field r)) } in H
+    | H: context[{ ?r with ?field := ?v }] |- _ =>
+        let h := head r in is_constructor h;
+        let res := apply_set r r field v in
+        progress change { r with field := v } with res in H
+    | H: context[{ ?r with ?field ::= ?f }] |- _ =>
+        let h := head r in is_constructor h;
+        let bare_field := head field in (* <-- strip implicit args/params *)
+        let oldval := eval cbn [bare_field] in (field r) in
+        let res := apply_set r r field (f oldval) in
+        progress change { r with field ::= f } with res in H
+    end.
+
+  Ltac simp := repeat simp_step.
+End record.
